LeanConcurrency/ConcurrencyImplementation.lean
@@ -7,10 +7,10 @@ open Concurrency
 open State
 
 -- simple concurrent example using a mutex to protect a shared abstract state.
-def runIO (nthreads : Nat := 3) (hn : nthreads > 0 := by omega) : IO Unit := do
+def runIO (nthreads : Nat := 3) (hN2 : 1 < nthreads := by omega) : IO Unit := do
   let N := nthreads
-  have inst : NeZero N := ⟨by omega⟩
-  let state : IO.Ref (State N) ← IO.mkRef State.init
+  let inst : NeZero N := ⟨Nat.ne_of_gt (Nat.lt_trans Nat.zero_lt_one hN2)⟩
+  let state : IO.Ref (@State N inst) ← IO.mkRef (@State.init N inst)
   let mutex : Std.Mutex Unit ← Std.Mutex.new ()
 
   let showBool : Bool -> String := fun
@@ -37,6 +37,7 @@ def runIO (nthreads : Nat := 3) (hn : nthreads > 0 := by omega) : IO Unit := do
 /-- refinement theorem: every reachable state satisfies the
 inductive invariant. -/
 theorem runIO_implements_invariants (nthreads : Nat) [NeZero nthreads]
+  (hN2 : 1 < nthreads)
     {st : State nthreads} :
     State.reachable st → State.InductiveInvariant st := by
   intro hreach
@@ -45,6 +46,6 @@ theorem runIO_implements_invariants (nthreads : Nat) [NeZero nthreads]
       intro p hy
       simp [State.init] at hy
   | step s t _ hstep ih =>
-      exact Concurrency.step_preserves_ind_inv hstep ih
+    exact Concurrency.step_preserves_ind_inv hstep ih hN2
 
 end LeanConcurrency.ConcurrencyImplementation
